add level chunk functions

crypto_examples/ntt.dfy
@@ -13,13 +13,46 @@ module ntt {
     import opened ntt_rec
     import opened rindex
 
-    function A(): seq<elem>
+    function method A(): seq<elem>
         ensures |A()| == N == pow2(L).full;
 
-    function Ar(): seq<elem>
+    function method Ar(): seq<elem>
         ensures |Ar()| == N == pow2(L).full;
         ensures forall i | 0 <= i < N ::
             Ar()[i] == A()[build_rev_index(i).v];
+
+    function method {:fuel 4} build_level_chunks(len: pow2_t): (cs: seq<seq<elem>>)
+        requires 1 <= len.exp <= L
+        ensures |cs| == pow2_div(pow2(L), len).full;
+        ensures forall i | 0 <= i < |cs| :: |cs[i]| == len.full
+        decreases L - len.exp
+    {
+        if len.exp == L then [A()]
+        else 
+            var a := build_level_chunks(pow2_double(len));
+            assert |a| == pow2(L - len.exp - 1).full by {
+                assert |a| == pow2(L).full / (pow2(len.exp + 1).full);
+                reveal Pow2();
+                assert len.exp + 1 <= L;
+                LemmaPowSubtracts(2, len.exp + 1, L);
+            }
+            assert |a| * 2 == pow2(L - len.exp).full by {
+                reveal Pow2();
+                LemmaPowAdds(2, L - len.exp - 1, 1);
+                LemmaPow1(2);
+            }
+            seq(|a| * 2, k requires 0 <= k < |a| * 2 => 
+                if k % 2 == 0 then even_indexed_terms(a[k/2], len)
+                else odd_indexed_terms(a[(k-1)/2], len))
+    }
+
+    function method get_level_chunk(len: pow2_t, ki: nat): (chunk: seq<elem>)
+        requires 1 <= len.exp <= L
+        requires ki < pow2_div(pow2(L), len).full;
+        ensures |chunk| == len.full
+    {
+        build_level_chunks(len)[ki]
+    }
 
     lemma index_bounded_lemma(
         j: nat, k: nat, ki: nat,
@@ -67,8 +100,9 @@ module ntt {
         requires a'[k] == modadd(u, t);
         requires a'[k+1] == modsub(u, t);
 
-        ensures a'[k] == poly_eval([Ar()[k], Ar()[k+1]], omega_nk(m, 0));
-        ensures a'[k+1] == poly_eval([Ar()[k], Ar()[k+1]], omega_nk(m, 1));
+        ensures a'[k] == poly_eval(Ar()[k..k+2], omega_nk(m, 0));
+        ensures a'[k+1] == poly_eval(Ar()[k..k+2], omega_nk(m, 1));
+        // ensures Ar()[k..k+2] == get_level_chunk();
     {
         // nth_root_lemma();
         pow2_basics(m);
@@ -80,11 +114,8 @@ module ntt {
 
         var even := Ar()[k..k+1];
         var odd := Ar()[k+1..k+2];
-        var chunk := [Ar()[k], Ar()[k+1]];
+        var chunk :=Ar()[k..k+2];
         assert chunk == even + odd;
-
-        assert Ar()[k] == A()[build_rev_index(k).v];
-        assert Ar()[k+1] == A()[build_rev_index(k+1).v];
 
         var original := orignal_index(ki, 0, m);
         assert original.v == k;
@@ -188,7 +219,7 @@ module ntt {
     //     var ki := 0;
 
     //     while (ki < pow2_div(pow2(L), m).full) 
-    //         // at level s, each chunck is 2 ** s big
+    //         // at level s, each chunk is 2 ** s big
     //         // invariant step_count == pow2_div(pow2(L), m);
     //         // invariant step_count.exp == L - m.exp;
     //         invariant 0 <= k == ki * m.full;
